\documentclass[]{article}
\usepackage[parfill]{parskip}
\usepackage{amsmath}
\title{Gompertz GLM Formulations}
\author{Sina Sajadmanesh}

\begin{document}

\maketitle

Gompertz distribution:
\[f_T(t)=\alpha e^t\exp\left\lbrace -\alpha(e^t-1) \right\rbrace\]
\[S(t)=\exp\left\lbrace -\alpha(e^t-1) \right\rbrace  \quad,\quad  \lambda(t)=\alpha e^t\]

GLM hypothesis:
\[\alpha=\exp(w^Tx)\]
Likelihood:
\begin{equation*}
\begin{split}
\mathcal{L}(D)=&\prod_{i=1}^{N}f_T(t_i\mid x_i)^{y_i}P(T\ge t_i\mid x_i)^{1-y_i}\\
=&\prod_{i=1}^{N}f_T(t_i\mid x_i)^{y_i}S(t_i\mid x_i)^{1-y_i}\\
=&\prod_{i=1}^{N}[\lambda(t_i\mid x_i)S(t_i\mid x_i)]^{y_i}S(t_i\mid x_i)^{1-y_i}\\
=&\prod_{i=1}^{N}\lambda(t_i\mid x_i)^{y_i}S(t_i\mid x_i)\\
=&\prod_{i=1}^{N}\left[\alpha_ie^{t_i}\right]^{y_i}\exp\left\lbrace -\alpha_i(e^{t_i}-1) \right\rbrace\\
=&\prod_{i=1}^{N}\exp(w^Tx_i+t_i)^{y_i}\exp\left\lbrace -\exp(w^Tx_i)(e^{t_i}-1) \right\rbrace\\
\end{split}
\end{equation*}

Log-likelihood:
\begin{equation*}
\begin{split}
\log\mathcal{L}(D)
=&\sum_{i=1}^{N}y_i[w^Tx_i+t_i]-\exp(w^Tx_i)(e^{t_i}-1)\\
\end{split}
\end{equation*}

With respect to $w$:
\begin{equation*}
\begin{split}
-\log\mathcal{L}(D)=&\sum_{i=1}^{N}\exp(w^Tx_i)(e^{t_i}-1)-y_iw^Tx_i\\
-\frac{\partial}{\partial w}\log\mathcal{L}(D)=&\sum_{i=1}^{N}x_i\left[\exp(w^Tx_i)(e^{t_i}-1)-y_i\right]\\
-\frac{\partial^2}{\partial w^2}\log\mathcal{L}(D)=&\sum_{i=1}^{N}x_ix_i^T\exp(w^Tx_i)(e^{t_i}-1)\\
\end{split}
\end{equation*}

\end{document}
